Clean/Orchard/Ecc.lean
@@ -71,6 +71,7 @@ def pallasScalarMulCoords (scalar : ℕ) (base : Point PallasBaseField) :
 
 inductive OrchardFixedBaseId where
   | commitIvkR
+  | noteCommitR
   | valueCommitV
   | valueCommitR
   | nullifierK
@@ -78,12 +79,15 @@ inductive OrchardFixedBaseId where
 deriving DecidableEq
 
 /- Coordinates copied from Orchard 0.14.0 fixed-base generators in
-`orchard/src/constants/fixed_bases/{commit_ivk_r,value_commit_v,value_commit_r,nullifier_k,spend_auth_g}.rs`.
+`orchard/src/constants/fixed_bases/{commit_ivk_r,note_commit_r,value_commit_v,value_commit_r,nullifier_k,spend_auth_g}.rs`.
 -/
 def fixedBasePoint : OrchardFixedBaseId → Point PallasBaseField
   | .commitIvkR =>
       { x := 17022113834174368664964072539940476916905682548990455171271428285673934201112,
         y := 18912017636736613471143674001158885358143653198146604093009134371854861983145 }
+  | .noteCommitR =>
+      { x := 17502433695644481444785977856966854265310331039772160001849803703443502427667,
+        y := 27531606546556235994383748883097777001194017792923801570415255878186539366371 }
   | .valueCommitV =>
       { x := 21457208314186520936880902219424053485005045883401337627148481900742711001959,
         y := 20379375922573002911833717643813254676246486412159279022689151936901102105230 }
